src/dvspec/dafny/dvn.dfy
@@ -1,0 +1,176 @@
+include "commons.dfy"
+include "dvc_spec.dfy"
+include "consensus.dfy"
+include "network.dfy"
+
+module DVC 
+{
+    import opened Types
+    import opened NetworkM
+    import opened ConsensusSpec
+    import opened DVCNode_Externs_Proofs
+    import opened DVCNode_Implementation_Helpers
+    import opened DVCNode = DVCNode_Implementation_Proofs`PublicInterface
+
+    datatype Adversary = Adversary(
+        nodes: set<BLSPubkey>
+    )
+
+    datatype DSVState = DSVState(
+        all_nodes: set<BLSPubkey>,
+        honest_nodes_states: map<BLSPubkey, DVCNodeState>,
+        adversary: Adversary,
+        dv_pubkey: BLSPubkey,
+        // attestations_shares_sent: set<AttestationShare>,
+        consensus_on_attestation_data: imaptotal<Slot, ConsensusInstance<AttestationData>>,
+        att_network: NetworkM.Network<AttestationShare>,
+        all_attestations_created: set<Attestation>,
+        slashing_dbs_used_for_validating_attestations: imaptotal<Slot, set<AttestationSlashingDB>>,
+        // aggregated_attestations_sent: set<Attestation>,
+        // attestation_duties_served: map<AttestationDuty, set<BLSPubkey>>,
+        construct_signed_attestation_signature: (set<AttestationShare>) -> Optional<BLSSignature>
+    )
+
+    datatype Event = 
+    | AdeversaryTakingStep(node: BLSPubkey, new_attestation_shares_sent: set<AttestationShare>,
+        messagesReceivedByTheNode: set<AttestationShare>)
+    | HonestNodeTakingStep(node: BLSPubkey, event: DVCNode.Event, nodeOutputs: DVCNode.Outputs)
+
+
+    predicate is_slashable_attestation_data(slashing_db: AttestationSlashingDB, attestation_data: AttestationData)
+
+    predicate Next(
+        s: DSVState,
+        s': DSVState 
+    )
+    {
+        exists e ::
+            NextEvent(s, e, s')
+    }
+
+    predicate NextEvent(
+        s: DSVState,
+        event: Event,
+        s': DSVState
+    )
+    {
+        && s'.honest_nodes_states.Keys == s.honest_nodes_states.Keys
+        && (
+            match event
+                case HonestNodeTakingStep(node, nodeEvent, nodeOutputs) => 
+                    && NextHonestNode(s, node, nodeEvent, nodeOutputs, s')
+                case AdeversaryTakingStep(node, new_attestation_share_sent, messagesReceivedByTheNode) => 
+                    NextAdversary(s, node, new_attestation_share_sent, messagesReceivedByTheNode, s')
+        )
+
+    }
+
+
+    predicate NextHonestNode(
+        s: DSVState,
+        node: BLSPubkey,
+        nodeEvent: DVCNode.Event,
+        nodeOutputs: DVCNode.Outputs,
+        s': DSVState
+    )
+    {
+        && s'.honest_nodes_states.Keys == s.honest_nodes_states.Keys
+        && s'.dv_pubkey == s.dv_pubkey        
+        && node in s.honest_nodes_states.Keys 
+        && var new_node_state := s'.honest_nodes_states[node];
+        && f_next(s.honest_nodes_states[node], nodeEvent, new_node_state, nodeOutputs)
+        && s'.honest_nodes_states == s.honest_nodes_states[
+            node := new_node_state
+        ]
+        && s'.all_attestations_created == s.all_attestations_created + nodeOutputs.attestations_submitted
+        && var messagesReceivedByTheNode :=
+            match nodeEvent
+                case ReceviedAttesttionShare(attestation_share) => {attestation_share}
+                case _ => {}
+            ;
+        && NetworkNext(s.att_network, s'.att_network, Some(node), nodeOutputs.att_shares_sent, messagesReceivedByTheNode)
+        && (
+                forall consensus_id: Slot ::
+                    s'.slashing_dbs_used_for_validating_attestations[consensus_id] == s.slashing_dbs_used_for_validating_attestations[consensus_id] +
+                        if isNodeRunning(s.consensus_on_attestation_data[consensus_id], node) then
+                            {s'.honest_nodes_states[node].attestation_slashing_db}
+                        else
+                            {}
+            )
+        && (
+            forall cid | cid in s.consensus_on_attestation_data.Keys ::
+                var inputCommands := set c | 
+                                    && c in nodeOutputs.att_consensus_commands_sent
+                                    && c.id == cid
+                            ::
+                                if c.Start? then 
+                                    Some(ConsensusSpec.Start(node))
+                                else
+                                    Some(ConsensusSpec.Stop(node));
+                var input :|
+                    if inputCommands == {} then
+                        input == None
+                    else
+                        input in inputCommands;
+
+                var output := 
+                    if nodeEvent.AttConsensusDecided? && nodeEvent.id == cid then 
+                        Some(Decided(node, nodeEvent.decided_attestation_data))
+                    else
+                        None
+                    ;
+
+                && var validityPredicate := 
+                    (ad: AttestationData) => 
+                        exists db | db in s.slashing_dbs_used_for_validating_attestations[cid] ::
+                            !is_slashable_attestation_data(db, ad)
+                    ;
+
+                ConsensusSpec.Next(
+                    s.consensus_on_attestation_data[cid],
+                    input,
+                    validityPredicate,
+                    s'.consensus_on_attestation_data[cid],
+                    output
+                )
+        )
+        && s'.adversary == s.adversary
+    }    
+
+    predicate NextAdversary(
+        s: DSVState,
+        node: BLSPubkey,
+        new_attestation_shares_sent: set<AttestationShare>,
+        messagesReceivedByTheNode: set<AttestationShare>,
+        s': DSVState
+    )
+    {
+
+        (
+            && node in (s.all_nodes - s.honest_nodes_states.Keys)
+            && (
+                forall new_attestation_share_sent, signer | new_attestation_share_sent in new_attestation_shares_sent ::
+                    verify_bls_siganture(new_attestation_share_sent.data, new_attestation_share_sent.signature, signer) ==> signer in s.adversary.nodes
+            )
+            && NetworkNext(s.att_network, s'.att_network, Some(node), new_attestation_shares_sent, messagesReceivedByTheNode)
+            && s.all_attestations_created <= s'.all_attestations_created
+            && var new_aggregated_attestations_sent := s'.all_attestations_created - s.all_attestations_created;
+            && (forall aggregated_attestation_sent | aggregated_attestation_sent in new_aggregated_attestations_sent ::
+                    exists attestation_shares ::
+                            && attestation_shares <= s'.att_network.allMessagesSent
+                            // && var sig_shares := set x | x in attestation_shares :: x.signature;
+                            && var constructed_sig := s.construct_signed_attestation_signature(attestation_shares);
+                            && constructed_sig.isPresent()
+                            && constructed_sig.safe_get() == aggregated_attestation_sent.signature
+            )
+            && s' == s.(
+                honest_nodes_states := s'.honest_nodes_states,
+                att_network := s'.att_network,
+                consensus_on_attestation_data := s'.consensus_on_attestation_data,
+                all_attestations_created := s'.all_attestations_created
+            )            
+        )         
+    }
+
+
+}
