src/dvspec/dafny/network.dfy
@@ -1,0 +1,68 @@
+include "commons.dfy"
+
+module NetworkM
+{
+    import opened Types
+    // import opened L1_SpecTypes
+
+    datatype Network<M> = Network(
+        messagesSentToNodeYetToBeReceived: map<BLSPubkey, multiset<M>>,
+        allMessagesSent: set<M>
+    )
+
+
+    predicate NetworkInit<M>(
+        e: Network<M>,
+        all_nodes: set<BLSPubkey>
+    )
+    {
+        && e.messagesSentToNodeYetToBeReceived.Keys == all_nodes
+        && forall v | v in e.messagesSentToNodeYetToBeReceived.Values :: v == multiset{}
+    }
+
+    predicate NetworkDeliverNext<M>(
+        e: Network<M>,
+        e': Network<M>,
+        n: BLSPubkey,
+        messagesToBeBroadcast: set<M>,
+        messagesReceived: set<M>
+    )
+    {
+        && e'.messagesSentToNodeYetToBeReceived.Keys == e.messagesSentToNodeYetToBeReceived.Keys
+        && n in e.messagesSentToNodeYetToBeReceived.Keys
+        && multiset(messagesReceived) <= e.messagesSentToNodeYetToBeReceived[n]
+        && |messagesReceived| <= 1
+        && e'.messagesSentToNodeYetToBeReceived == e.messagesSentToNodeYetToBeReceived[
+            n := e.messagesSentToNodeYetToBeReceived[n] - multiset(messagesReceived) + multiset(messagesToBeBroadcast)
+        ]
+        && e'.allMessagesSent == e.allMessagesSent + messagesToBeBroadcast
+    }
+
+    // predicate NetworkStutter(
+    //     e: Network,
+    //     e': Network
+    // )
+    // {
+    //     e' == e
+    // }
+
+    predicate NetworkNext<M>(
+        e: Network,
+        e': Network,
+        n : Optional<BLSPubkey>,
+        messagesSentByTheNodes: set<M>,
+        messagesReceivedByTheNodes: set<M>
+    )
+    {
+        || (
+            && n.isPresent()
+            && NetworkDeliverNext(e, e', n.safe_get(), messagesSentByTheNodes,messagesReceivedByTheNodes)
+        )
+        // || (
+        //     && !n.isPresent()
+        //     && NetworkStutter(e, e')
+        //     && messagesSentByTheNodes == {}
+        //     && messagesReceivedByTheNodes == {}
+        // )
+    }
+}
